Finally get through the transfer from basic stepping to bir exec to labels...

src/tools/symbexec/examples/analysis/motorfunc_transfScript.sml
@@ -305,7 +305,7 @@ val tm = ``
 
 birs_symb_symbols_CONV tm
 
-val tm2 = ``birs_exps_of_senv_COMP ∅
+val tm2 = ``birs_exps_of_senv_COMP {} 
              (K NONE)⦇
                "countw" ↦
                  SOME
@@ -340,7 +340,7 @@ val tm2 = ``birs_exps_of_senv_COMP ∅
                "countw" ↦
                  SOME (BExp_Den (BVar "sy_countw" (BType_Imm Bit64)))
              ⦈``;
-val tm2 = ``birs_exps_of_senv_COMP ∅
+val tm2 = ``birs_exps_of_senv_COMP {} 
              (K NONE)⦇
                "countw" ↦
                  SOME
@@ -486,10 +486,1072 @@ val bprog_bir_prop_thm = save_thm(
 );
 (* ........................... *)
 
+val bir_step_n_in_L_jgmt_def = Define `
+    bir_step_n_in_L_jgmt bprog l L pre post =
+ !st.
+   (st.bst_pc = l) ==>
+   (pre st) ==>
+   (?n st'.
+     (step_n_in_L (\x. x.bst_pc) (bir_exec_step_state bprog) st n L st') /\
+     (post st st'))
+`;
+
+val bir_step_n_in_L_jgmt_thm = prove(``
+(bir_step_n_in_L_jgmt
+  bprog
+  <|bpc_label := BL_Address (Imm32 2824w); bpc_index := 0|>
+  motor_analysis_L
+  (\st.
+       st.bst_status = BST_Running /\
+       bir_envty_list_b birenvtyl st.bst_environ /\
+       bir_eval_exp
+         (BExp_BinExp BIExp_And
+            (BExp_BinExp BIExp_And
+               (BExp_BinPred BIExp_LessOrEqual (BExp_Const (Imm32 0xFFFFFFw))
+                  (BExp_Den (BVar "SP_process" (BType_Imm Bit32))))
+               (BExp_Aligned Bit32 2
+                  (BExp_Den (BVar "SP_process" (BType_Imm Bit32)))))
+            (BExp_BinPred BIExp_LessOrEqual
+               (BExp_Den (BVar "countw" (BType_Imm Bit64)))
+               (BExp_Const (Imm64 0xFFFFFFFFFFFFFF00w)))) st.bst_environ =
+       SOME bir_val_true)
+  (\st st'.
+         (st'.bst_pc = <|bpc_label := BL_Address (Imm32 2886w); bpc_index := 0|>) /\
+         ?v1 v2.
+           bir_env_lookup "countw" st.bst_environ =
+           SOME (BVal_Imm (Imm64 v1)) /\
+           bir_env_lookup "countw" st'.bst_environ =
+           SOME (BVal_Imm (Imm64 v2)) /\
+           v1 <+ v2 /\
+           v1 + 44w <=+ v2 /\
+           v2 <=+ v1 + 47w))
+``,
+  cheat
+);
 
 
+
+local
+  open bir_programTheory;
+  open bir_inst_liftingTheory;
+
+  val bir_state_ss = rewrites (type_rws ``:bir_state_t``);
+in
+
+
+val bir_exec_stmtB_INIT_FINAL_Running_thm = store_thm(
+   "bir_exec_stmtB_INIT_FINAL_Running_thm", ``
+!stmt bs bs'.
+  (SND (bir_exec_stmtB stmt bs) = bs') ==>
+  (bs.bst_status = BST_Running) ==>
+  (bs'.bst_status = BST_Running \/ (bs.bst_pc = bs'.bst_pc))
+``,
+  REPEAT GEN_TAC >>
+  DISCH_TAC >>
+
+  Cases_on `stmt` >- (
+    FULL_SIMP_TAC (std_ss++bir_state_ss++holBACore_ss) [bir_exec_stmtB_def, bir_exec_stmt_assign_def] >>
+    Cases_on `bir_eval_exp b0 bs.bst_environ` >- (
+      ASSUME_TAC (Q.SPEC `bs` bir_state_t_literal_nchotomy) >>
+      ASSUME_TAC (Q.SPEC `bs'` bir_state_t_literal_nchotomy) >>
+
+      FULL_SIMP_TAC (std_ss++bir_state_ss++holBACore_ss) [bir_state_set_typeerror_def] >>
+      FULL_SIMP_TAC (std_ss++bir_state_ss++holBACore_ss) []
+    ) >>
+
+    FULL_SIMP_TAC (std_ss++bir_state_ss++holBACore_ss) [] >>
+    Cases_on `bir_env_write b x bs.bst_environ` >> (
+      ASSUME_TAC (Q.SPEC `bs` bir_state_t_literal_nchotomy) >>
+      ASSUME_TAC (Q.SPEC `bs'` bir_state_t_literal_nchotomy) >>
+
+      FULL_SIMP_TAC (std_ss++bir_state_ss++holBACore_ss) [bir_state_set_typeerror_def] >>
+      FULL_SIMP_TAC (std_ss++bir_state_ss++holBACore_ss) []
+    )
+  ) >- (
+    FULL_SIMP_TAC (std_ss++bir_state_ss++holBACore_ss) [bir_exec_stmtB_def, bir_exec_stmt_assert_def] >>
+    Cases_on `bir_eval_exp b bs.bst_environ` >- (
+      ASSUME_TAC (Q.SPEC `bs` bir_state_t_literal_nchotomy) >>
+      ASSUME_TAC (Q.SPEC `bs'` bir_state_t_literal_nchotomy) >>
+
+      FULL_SIMP_TAC (std_ss++bir_state_ss++holBACore_ss) [bir_state_set_typeerror_def] >>
+      FULL_SIMP_TAC (std_ss++bir_state_ss++holBACore_ss) []
+    ) >>
+
+    FULL_SIMP_TAC (std_ss++bir_state_ss++holBACore_ss) [] >>
+    Cases_on `bir_dest_bool_val x` >- (
+      ASSUME_TAC (Q.SPEC `bs` bir_state_t_literal_nchotomy) >>
+      ASSUME_TAC (Q.SPEC `bs'` bir_state_t_literal_nchotomy) >>
+
+      FULL_SIMP_TAC (std_ss++bir_state_ss++holBACore_ss) [bir_state_set_typeerror_def] >>
+      FULL_SIMP_TAC (std_ss++bir_state_ss++holBACore_ss) []
+    ) >>
+
+    Cases_on `x'` >> (
+      ASSUME_TAC (Q.SPEC `bs` bir_state_t_literal_nchotomy) >>
+      ASSUME_TAC (Q.SPEC `bs'` bir_state_t_literal_nchotomy) >>
+
+      FULL_SIMP_TAC (std_ss++bir_state_ss++holBACore_ss) [bir_state_set_typeerror_def] >>
+      FULL_SIMP_TAC (std_ss++bir_state_ss++holBACore_ss) []
+    )
+  ) >- (
+    FULL_SIMP_TAC (std_ss++bir_state_ss++holBACore_ss) [bir_exec_stmtB_def, bir_exec_stmt_assume_def] >>
+    Cases_on `bir_eval_exp b bs.bst_environ` >- (
+      ASSUME_TAC (Q.SPEC `bs` bir_state_t_literal_nchotomy) >>
+      ASSUME_TAC (Q.SPEC `bs'` bir_state_t_literal_nchotomy) >>
+
+      FULL_SIMP_TAC (std_ss++bir_state_ss++holBACore_ss) [bir_state_set_typeerror_def] >>
+      FULL_SIMP_TAC (std_ss++bir_state_ss++holBACore_ss) []
+    ) >>
+
+    FULL_SIMP_TAC (std_ss++bir_state_ss++holBACore_ss) [] >>
+    Cases_on `bir_dest_bool_val x` >- (
+      ASSUME_TAC (Q.SPEC `bs` bir_state_t_literal_nchotomy) >>
+      ASSUME_TAC (Q.SPEC `bs'` bir_state_t_literal_nchotomy) >>
+
+      FULL_SIMP_TAC (std_ss++bir_state_ss++holBACore_ss) [bir_state_set_typeerror_def] >>
+      FULL_SIMP_TAC (std_ss++bir_state_ss++holBACore_ss) []
+    ) >>
+
+    Cases_on `x'` >> (
+      ASSUME_TAC (Q.SPEC `bs` bir_state_t_literal_nchotomy) >>
+      ASSUME_TAC (Q.SPEC `bs'` bir_state_t_literal_nchotomy) >>
+
+      FULL_SIMP_TAC (std_ss++bir_state_ss++holBACore_ss) [bir_state_set_typeerror_def] >>
+      FULL_SIMP_TAC (std_ss++bir_state_ss++holBACore_ss) []
+    )
+  ) >>
+
+  FULL_SIMP_TAC (std_ss++bir_state_ss++holBACore_ss) [bir_exec_stmtB_def, bir_exec_stmt_observe_def] >>
+  Q.ABBREV_TAC `A = MAP (\e. bir_eval_exp e bs.bst_environ) l` >>
+  FULL_SIMP_TAC (std_ss++bir_state_ss++holBACore_ss) [LET_DEF] >>
+
+  Cases_on `bir_eval_exp b bs.bst_environ` >- (
+    ASSUME_TAC (Q.SPEC `bs` bir_state_t_literal_nchotomy) >>
+    ASSUME_TAC (Q.SPEC `bs'` bir_state_t_literal_nchotomy) >>
+
+    FULL_SIMP_TAC (std_ss++bir_state_ss++holBACore_ss) [bir_state_set_typeerror_def] >>
+    FULL_SIMP_TAC (std_ss++bir_state_ss++holBACore_ss) []
+  ) >>
+
+  FULL_SIMP_TAC (std_ss++bir_state_ss++holBACore_ss) [] >>
+  Cases_on `bir_dest_bool_val x` >- (
+    ASSUME_TAC (Q.SPEC `bs` bir_state_t_literal_nchotomy) >>
+    ASSUME_TAC (Q.SPEC `bs'` bir_state_t_literal_nchotomy) >>
+
+    FULL_SIMP_TAC (std_ss++bir_state_ss++holBACore_ss) [bir_state_set_typeerror_def] >>
+    FULL_SIMP_TAC (std_ss++bir_state_ss++holBACore_ss) []
+  ) >>
+
+  FULL_SIMP_TAC (std_ss++bir_state_ss++holBACore_ss) [] >>
+  Cases_on `x'` >> Cases_on `EXISTS IS_NONE A` >> (
+    ASSUME_TAC (Q.SPEC `bs` bir_state_t_literal_nchotomy) >>
+    ASSUME_TAC (Q.SPEC `bs'` bir_state_t_literal_nchotomy) >>
+
+    FULL_SIMP_TAC (std_ss++bir_state_ss++holBACore_ss) [bir_state_set_typeerror_def] >>
+    FULL_SIMP_TAC (std_ss++bir_state_ss++holBACore_ss) []
+  )
+);
+
+
+val bir_exec_stmt_jmp_to_label_INIT_FINAL_Running_thm = store_thm(
+   "bir_exec_stmt_jmp_to_label_INIT_FINAL_Running_thm", ``
+!p l bs bs'.
+  (bir_exec_stmt_jmp_to_label p l bs = bs') ==>
+  (bs.bst_status = BST_Running) ==>
+  (bs'.bst_status = BST_Running \/ (bs.bst_pc = bs'.bst_pc))
+``,
+  REPEAT STRIP_TAC >>
+
+  FULL_SIMP_TAC (std_ss++bir_state_ss++holBACore_ss) [bir_exec_stmt_jmp_to_label_def] >>
+  Cases_on `MEM l (bir_labels_of_program p)` >- (
+    ASSUME_TAC (Q.SPEC `bs` bir_state_t_literal_nchotomy) >>
+    ASSUME_TAC (Q.SPEC `bs'` bir_state_t_literal_nchotomy) >>
+
+    FULL_SIMP_TAC (std_ss++bir_state_ss++holBACore_ss) [bir_state_set_typeerror_def] >>
+    FULL_SIMP_TAC (std_ss++bir_state_ss++holBACore_ss) []
+  ) >>
+
+  ASSUME_TAC (Q.SPEC `bs` bir_state_t_literal_nchotomy) >>
+  ASSUME_TAC (Q.SPEC `bs'` bir_state_t_literal_nchotomy) >>
+
+  FULL_SIMP_TAC (std_ss++bir_state_ss++holBACore_ss) [bir_state_set_typeerror_def] >>
+  FULL_SIMP_TAC (std_ss++bir_state_ss++holBACore_ss) []
+);
+
+
+val bir_exec_stmt_jmp_INIT_FINAL_Running_thm = store_thm(
+   "bir_exec_stmt_jmp_INIT_FINAL_Running_thm", ``
+!p le bs bs'.
+  (bir_exec_stmt_jmp p le bs = bs') ==>
+  (bs.bst_status = BST_Running) ==>
+  (bs'.bst_status = BST_Running \/ (bs.bst_pc = bs'.bst_pc))
+``,
+  REPEAT GEN_TAC >>
+  DISCH_TAC >>
+
+    FULL_SIMP_TAC (std_ss++bir_state_ss++holBACore_ss) [bir_exec_stmt_jmp_def] >>
+    Cases_on `bir_eval_label_exp le bs.bst_environ` >- (
+      ASSUME_TAC (Q.SPEC `bs` bir_state_t_literal_nchotomy) >>
+      ASSUME_TAC (Q.SPEC `bs'` bir_state_t_literal_nchotomy) >>
+      FULL_SIMP_TAC (std_ss++bir_state_ss++holBACore_ss) [bir_state_set_typeerror_def] >>
+      FULL_SIMP_TAC (std_ss++bir_state_ss++holBACore_ss) [] >>
+      METIS_TAC [bir_status_t_distinct]
+    ) >>
+
+    FULL_SIMP_TAC (std_ss++bir_state_ss++holBACore_ss) [] >>
+    METIS_TAC [bir_exec_stmt_jmp_to_label_INIT_FINAL_Running_thm]
+);
+
+val bir_exec_stmtE_INIT_FINAL_Running_thm = store_thm(
+   "bir_exec_stmtE_INIT_FINAL_Running_thm", ``
+!p estmt bs bs'.
+  (bir_exec_stmtE p estmt bs = bs') ==>
+  (bs.bst_status = BST_Running) ==>
+  ((bs.bst_pc <> bs'.bst_pc) ==> (bs'.bst_status = BST_Running))
+``,
+  REPEAT GEN_TAC >>
+  DISCH_TAC >>
+
+  Cases_on `estmt` >- (
+    FULL_SIMP_TAC (std_ss++bir_state_ss++holBACore_ss) [bir_exec_stmtE_def] >>
+    METIS_TAC [bir_exec_stmt_jmp_INIT_FINAL_Running_thm]
+  ) >- (
+    FULL_SIMP_TAC (std_ss++bir_state_ss++holBACore_ss) [bir_exec_stmtE_def, bir_exec_stmt_cjmp_def] >>
+    Cases_on `bir_eval_exp b bs.bst_environ` >- (
+      ASSUME_TAC (Q.SPEC `bs` bir_state_t_literal_nchotomy) >>
+      ASSUME_TAC (Q.SPEC `bs'` bir_state_t_literal_nchotomy) >>
+      FULL_SIMP_TAC (std_ss++bir_state_ss++holBACore_ss) [bir_state_set_typeerror_def, LET_DEF] >>
+      FULL_SIMP_TAC (std_ss++bir_state_ss++holBACore_ss) []
+    ) >>
+
+    FULL_SIMP_TAC (std_ss++bir_state_ss++holBACore_ss) [LET_DEF] >>
+    Cases_on `bir_dest_bool_val x` >- (
+      ASSUME_TAC (Q.SPEC `bs` bir_state_t_literal_nchotomy) >>
+      ASSUME_TAC (Q.SPEC `bs'` bir_state_t_literal_nchotomy) >>
+      FULL_SIMP_TAC (std_ss++bir_state_ss++holBACore_ss) [bir_state_set_typeerror_def, LET_DEF] >>
+      FULL_SIMP_TAC (std_ss++bir_state_ss++holBACore_ss) []
+    ) >>
+
+    Cases_on `x'` >> (
+      FULL_SIMP_TAC (std_ss++bir_state_ss++holBACore_ss) [] >>
+      METIS_TAC [bir_exec_stmt_jmp_INIT_FINAL_Running_thm]
+    )
+  ) >>
+
+  FULL_SIMP_TAC (std_ss++bir_state_ss++holBACore_ss) [bir_exec_stmtE_def, bir_exec_stmt_halt_def] >>
+  Cases_on `bir_eval_exp b bs.bst_environ` >- (
+      ASSUME_TAC (Q.SPEC `bs` bir_state_t_literal_nchotomy) >>
+      ASSUME_TAC (Q.SPEC `bs'` bir_state_t_literal_nchotomy) >>
+      FULL_SIMP_TAC (std_ss++bir_state_ss++holBACore_ss) [bir_state_set_typeerror_def, LET_DEF] >>
+      FULL_SIMP_TAC (std_ss++bir_state_ss++holBACore_ss) []
+  ) >>
+
+  ASSUME_TAC (Q.SPEC `bs` bir_state_t_literal_nchotomy) >>
+  ASSUME_TAC (Q.SPEC `bs'` bir_state_t_literal_nchotomy) >>
+  FULL_SIMP_TAC (std_ss++bir_state_ss++holBACore_ss) [bir_state_set_typeerror_def, LET_DEF] >>
+  FULL_SIMP_TAC (std_ss++bir_state_ss++holBACore_ss) []
+);
+
+
+val bir_exec_step_INIT_FINAL_Running_thm = store_thm(
+   "bir_exec_step_INIT_FINAL_Running_thm", ``
+!p bs bs'.
+  (SND (bir_exec_step p bs) = bs') ==>
+  (((bs.bst_pc <> bs'.bst_pc) ==> (bs'.bst_status = BST_Running)) /\
+   ((bs'.bst_status = BST_Running) ==> (bs.bst_status = BST_Running)))
+``,
+  REPEAT GEN_TAC >>
+  DISCH_TAC >>
+  FULL_SIMP_TAC (std_ss++holBACore_ss) [bir_exec_step_def] >>
+  Cases_on `bir_state_is_terminated bs` >> (
+    FULL_SIMP_TAC (std_ss++holBACore_ss) []
+  ) >>
+  Cases_on `bir_get_current_statement p bs.bst_pc` >- (
+    ASSUME_TAC (Q.SPEC `bs` bir_state_t_literal_nchotomy) >>
+    ASSUME_TAC (Q.SPEC `bs'` bir_state_t_literal_nchotomy) >>
+    FULL_SIMP_TAC (std_ss++bir_state_ss++holBACore_ss) [bir_state_set_failed_def, bir_state_is_terminated_def] >>
+    FULL_SIMP_TAC (std_ss++bir_state_ss++holBACore_ss) []
+  ) >>
+
+  FULL_SIMP_TAC (std_ss++holBACore_ss) [] >>
+
+  Cases_on `x` >- (
+    FULL_SIMP_TAC (std_ss++bir_state_ss++holBACore_ss) [bir_exec_stmt_def] >>
+    Cases_on `bir_exec_stmtB b bs` >>
+    FULL_SIMP_TAC (std_ss++bir_state_ss++holBACore_ss) [LET_DEF] >>
+
+    Cases_on `bir_state_is_terminated r` >- (
+      FULL_SIMP_TAC (std_ss++bir_state_ss++holBACore_ss) [bir_state_set_failed_def, bir_state_is_terminated_def] >>
+      METIS_TAC [bir_exec_stmtB_INIT_FINAL_Running_thm, pairTheory.SND]
+    ) >>
+    FULL_SIMP_TAC (std_ss++bir_state_ss++holBACore_ss) [bir_state_set_failed_def, bir_state_is_terminated_def] >>
+    ASSUME_TAC (Q.SPEC `r` bir_state_t_literal_nchotomy) >>
+    ASSUME_TAC (Q.SPEC `bs'` bir_state_t_literal_nchotomy) >>
+    FULL_SIMP_TAC (std_ss++bir_state_ss++holBACore_ss) [] >>
+    FULL_SIMP_TAC (std_ss++bir_state_ss++holBACore_ss) []
+  ) >>
+
+  FULL_SIMP_TAC (std_ss++bir_state_ss++holBACore_ss) [bir_exec_stmt_def, bir_state_is_terminated_def] >>
+  IMP_RES_TAC bir_exec_stmtE_INIT_FINAL_Running_thm
+);
+
+val bir_exec_step_state_PC_DIFF_IMP_FINAL_Running_thm = store_thm(
+   "bir_exec_step_state_PC_DIFF_IMP_FINAL_Running_thm", ``
+!bprog bs bs'.
+  (bir_exec_step_state bprog bs = bs') ==>
+  (bs.bst_pc <> bs'.bst_pc) ==>
+  (bs'.bst_status = BST_Running)
+``,
+  REPEAT STRIP_TAC >>
+  FULL_SIMP_TAC (std_ss++holBACore_ss) [bir_exec_step_state_def] >>
+  IMP_RES_TAC bir_exec_step_INIT_FINAL_Running_thm
+);
+
+val bir_exec_step_state_FINAL_Running_IMP_INITIAL_Running_thm = store_thm(
+   "bir_exec_step_state_FINAL_Running_IMP_INITIAL_Running_thm", ``
+!bprog bs bs'.
+  (bir_exec_step_state bprog bs = bs') ==>
+  (bs'.bst_status = BST_Running) ==>
+  (bs.bst_status = BST_Running)
+``,
+  REPEAT STRIP_TAC >>
+  FULL_SIMP_TAC (std_ss++holBACore_ss) [bir_exec_step_state_def] >>
+  IMP_RES_TAC bir_exec_step_INIT_FINAL_Running_thm
+);
+
+
+(*
+val _thm = store_thm(
+   "_thm", ``
+!.
+  (bir_exec_steps_GEN (cfst, pcls) p st (SOME n) = BER_Ended lo i n' bs') ==>
+  (bs'.bst_status = BST_Running) ==>
+  ()
+``,
+  cheat
+);
+*)
+
+(*
+listTheory.REVERSE_GENLIST
+
+val GENLISTREV_def = Define `
+    GENLISTREV f n = 
+`;
+
+listTheory.GENLIST
+
+
+val _thm = store_thm(
+   "_thm", ``
+!p st n.
+  (GENLIST (\x. f (SUC x)) n)
+``,
+  cheat
+);
+*)
+
+val GENLIST_FUN_SUC_EQ_thm = store_thm(
+   "GENLIST_FUN_SUC_EQ_thm", ``
+!f g n.
+  (!m. (m <= n) ==> (f m = g m)) ==>
+  (GENLIST f (SUC n) =
+   GENLIST g (SUC n))
+``,
+  Induct_on `n` >> (
+    FULL_SIMP_TAC (std_ss++listSimps.LIST_ss) []
+  ) >>
+
+  REPEAT STRIP_TAC >>
+  PAT_X_ASSUM ``!x y. A`` (ASSUME_TAC o Q.SPECL [`f`, `g`]) >>
+
+  `!m. m <= n ==> f m = g m` by (
+    REPEAT STRIP_TAC >>
+    PAT_X_ASSUM ``!x. A`` (ASSUME_TAC o Q.SPEC `m`) >>
+    FULL_SIMP_TAC arith_ss []
+  ) >>
+  FULL_SIMP_TAC std_ss [listTheory.GENLIST]
+);
+
+val GENLIST_FUN_SUC_SUB_EQ_thm = store_thm(
+   "GENLIST_FUN_SUC_SUB_EQ_thm", ``
+!f n.
+  GENLIST (\m. f (SUC (n - m))) (SUC n) =
+  GENLIST (\m. f (SUC  n - m )) (SUC n)
+``,
+  REPEAT STRIP_TAC >>
+  MATCH_MP_TAC GENLIST_FUN_SUC_EQ_thm >>
+
+  REPEAT STRIP_TAC >>
+  FULL_SIMP_TAC std_ss [] >>
+
+  FULL_SIMP_TAC std_ss [arithmeticTheory.SUB_LEFT_SUC] >>
+
+  Cases_on `m = n` >- (
+    FULL_SIMP_TAC std_ss [arithmeticTheory.SUC_SUB]
+  ) >>
+
+  FULL_SIMP_TAC arith_ss []
+);
+
+val bir_exec_infinite_steps_fun_COMM_thm = store_thm(
+   "bir_exec_infinite_steps_fun_COMM_thm", ``
+!p st n.
+  (bir_exec_infinite_steps_fun p (bir_exec_step_state p st) n = bir_exec_step_state p (bir_exec_infinite_steps_fun p st n))
+``,
+  FULL_SIMP_TAC std_ss [bir_exec_infinite_steps_fun_def] >>
+
+  METIS_TAC [arithmeticTheory.FUNPOW, arithmeticTheory.FUNPOW_SUC]
+);
+
+val bir_exec_infinite_steps_fun_COUNT_PCs_SUC_MAP_ALT_thm = store_thm(
+   "bir_exec_infinite_steps_fun_COUNT_PCs_SUC_MAP_ALT_thm", ``
+!pc_cond bprog bs n.
+  (bir_exec_infinite_steps_fun_COUNT_PCs pc_cond bprog bs (SUC n) =
+   SUM (MAP (\x. if bir_state_COUNT_PC pc_cond x then 1 else 0) (REVERSE (GENLIST (\y. bir_exec_infinite_steps_fun bprog bs (SUC y)) (SUC n)))))
+``,
+  Induct_on `n` >- (
+    FULL_SIMP_TAC std_ss [bir_exec_infinite_steps_fun_COUNT_PCs_def, LET_DEF] >>
+    FULL_SIMP_TAC (std_ss++listSimps.LIST_ss) [] >>
+    SIMP_TAC std_ss [REWRITE_CONV [arithmeticTheory.ONE, bir_exec_infinite_steps_fun_REWRS] ``bir_exec_infinite_steps_fun bprog' bs 1``]
+  ) >>
+
+  REPEAT STRIP_TAC >>
+  SIMP_TAC std_ss [Once bir_exec_infinite_steps_fun_COUNT_PCs_def] >>
+  ASM_SIMP_TAC pure_ss [] >>
+  REWRITE_TAC [listTheory.REVERSE_GENLIST] >>
+  POP_ASSUM (K ALL_TAC) >>
+
+  REWRITE_TAC [GSYM (CONJUNCT2 bir_exec_infinite_steps_fun_REWRS)] >>
+
+  CONV_TAC (RAND_CONV (SIMP_CONV (pure_ss) [Once listTheory.GENLIST])) >>
+  SIMP_TAC std_ss [listTheory.MAP_SNOC, listTheory.SUM_SNOC] >>
+  SIMP_TAC std_ss [REWRITE_CONV [arithmeticTheory.ONE, bir_exec_infinite_steps_fun_REWRS] ``bir_exec_infinite_steps_fun bprog' bs 1``] >>
+
+  SIMP_TAC std_ss [
+   prove(
+    ``GENLIST (\m.  bir_exec_infinite_steps_fun bprog' bs (SUC (SUC (n - m)))) (SUC n) =
+      GENLIST (\m.  bir_exec_infinite_steps_fun bprog' bs (SUC (SUC  n - m ))) (SUC n)``,
+    FULL_SIMP_TAC std_ss [GENLIST_FUN_SUC_SUB_EQ_thm]
+   )]>>
+
+  CASE_TAC >> (
+    FULL_SIMP_TAC std_ss [LET_DEF, arithmeticTheory.ADD1]
+  )
+);
+
+val bir_exec_infinite_steps_fun_COUNT_PCs_ALT_def = Define `
+   (bir_exec_infinite_steps_fun_COUNT_PCs_ALT pc_cond bprog bs 0 = 0) /\
+   (bir_exec_infinite_steps_fun_COUNT_PCs_ALT pc_cond bprog bs (SUC n) = 
+    let
+      r = bir_exec_infinite_steps_fun_COUNT_PCs_ALT pc_cond bprog bs n
+    in
+      if bir_state_COUNT_PC pc_cond (bir_exec_infinite_steps_fun bprog bs (SUC n)) then
+        SUC r
+      else
+        r)
+`;
+
+val bir_exec_infinite_steps_fun_COUNT_PCs_ALT_thm = store_thm(
+   "bir_exec_infinite_steps_fun_COUNT_PCs_ALT_thm", ``
+  bir_exec_infinite_steps_fun_COUNT_PCs =
+  bir_exec_infinite_steps_fun_COUNT_PCs_ALT
+``,
+  REPEAT (MATCH_MP_TAC boolTheory.EQ_EXT >> GEN_TAC) >>
+  rename1 `bir_exec_infinite_steps_fun_COUNT_PCs pc_cond p bs n` >>
+
+  Cases_on `n` >- (
+    REWRITE_TAC [bir_exec_infinite_steps_fun_COUNT_PCs_ALT_def, bir_exec_infinite_steps_fun_COUNT_PCs_def]
+  ) >>
+
+  REWRITE_TAC [bir_exec_infinite_steps_fun_COUNT_PCs_SUC_MAP_ALT_thm] >>
+  REWRITE_TAC [rich_listTheory.MAP_REVERSE, rich_listTheory.SUM_REVERSE] >>
+  REWRITE_TAC [bir_exec_infinite_steps_fun_COUNT_PCs_ALT_def] >>
+
+  Induct_on `n'` >- (
+    FULL_SIMP_TAC std_ss [bir_exec_infinite_steps_fun_COUNT_PCs_def, LET_DEF] >>
+    FULL_SIMP_TAC (std_ss++listSimps.LIST_ss) [bir_exec_infinite_steps_fun_COUNT_PCs_ALT_def]
+  ) >>
+
+  SIMP_TAC (pure_ss) [Once listTheory.GENLIST] >>
+  SIMP_TAC pure_ss [listTheory.MAP_SNOC, listTheory.SUM_SNOC] >>
+  ASM_SIMP_TAC pure_ss [] >>
+
+  SIMP_TAC std_ss [GSYM bir_exec_infinite_steps_fun_COUNT_PCs_ALT_def] >>
+  POP_ASSUM (K ALL_TAC) >>
+  CONV_TAC (RAND_CONV (SIMP_CONV (pure_ss) [Once bir_exec_infinite_steps_fun_COUNT_PCs_ALT_def])) >>
+
+  CASE_TAC >> (
+    FULL_SIMP_TAC std_ss [LET_DEF, arithmeticTheory.ADD1]
+  )
+);
+
+val bir_exec_infinite_steps_fun_COUNT_PCs_LAST_STEP_thm = store_thm(
+   "bir_exec_infinite_steps_fun_COUNT_PCs_LAST_STEP_thm", ``
+!pc_cond bprog bs n.
+  (bir_state_COUNT_PC pc_cond (bir_exec_infinite_steps_fun bprog bs (SUC n))) ==>
+  (bir_exec_infinite_steps_fun_COUNT_PCs pc_cond bprog bs (SUC n) =
+   SUC (bir_exec_infinite_steps_fun_COUNT_PCs pc_cond bprog bs n))
+``,
+  FULL_SIMP_TAC std_ss [bir_exec_infinite_steps_fun_COUNT_PCs_ALT_thm, bir_exec_infinite_steps_fun_COUNT_PCs_ALT_def, LET_DEF]
+);
+
+val bir_exec_infinite_steps_fun_COUNT_PCs_GROWS_thm = store_thm(
+   "bir_exec_infinite_steps_fun_COUNT_PCs_GROWS_thm", ``
+!pc_cond bprog bs n n'.
+    (n' < n) ==>
+    (bir_exec_infinite_steps_fun_COUNT_PCs pc_cond bprog bs n' <= bir_exec_infinite_steps_fun_COUNT_PCs pc_cond bprog bs n)
+``,
+  Induct_on `n` >- (
+    FULL_SIMP_TAC arith_ss []
+  ) >>
+
+  REPEAT STRIP_TAC >>
+  Cases_on `n' = n` >- (
+    FULL_SIMP_TAC (std_ss) [bir_exec_infinite_steps_fun_COUNT_PCs_ALT_thm] >>
+    FULL_SIMP_TAC (std_ss) [bir_exec_infinite_steps_fun_COUNT_PCs_ALT_def, LET_DEF] >>
+    Cases_on `bir_state_COUNT_PC pc_cond (bir_exec_infinite_steps_fun bprog' bs (SUC n))` >> (
+      FULL_SIMP_TAC arith_ss []
+    )
+  ) >>
+  `n' < n` by (
+    FULL_SIMP_TAC arith_ss []
+  ) >>
+
+  PAT_X_ASSUM ``!x.A`` (ASSUME_TAC o Q.SPECL [`pc_cond`, `bprog'`, `bs`, `n'`]) >>
+  REV_FULL_SIMP_TAC std_ss [] >>
+
+  FULL_SIMP_TAC (std_ss) [bir_exec_infinite_steps_fun_COUNT_PCs_ALT_thm] >>
+  FULL_SIMP_TAC (std_ss) [bir_exec_infinite_steps_fun_COUNT_PCs_ALT_def, LET_DEF] >>
+
+  Cases_on `bir_state_COUNT_PC pc_cond (bir_exec_infinite_steps_fun bprog' bs (SUC n))` >> (
+    FULL_SIMP_TAC arith_ss []
+  )
+);
+
+
+val bir_exec_infinite_steps_fun_COUNT_PCs_LESS_STEPS_IMP_thm = store_thm(
+   "bir_exec_infinite_steps_fun_COUNT_PCs_LESS_STEPS_IMP_thm", ``
+!pc_cond bprog bs n k.
+  (bir_state_COUNT_PC pc_cond (bir_exec_infinite_steps_fun bprog bs n)) ==>
+  (bir_exec_infinite_steps_fun_COUNT_PCs pc_cond bprog bs n = k) ==>
+  (!n'.
+    (n' < n) ==>
+    (bir_exec_infinite_steps_fun_COUNT_PCs pc_cond bprog bs n' < k))
+``,
+  REPEAT STRIP_TAC >>
+
+  Cases_on `n` >- (
+    FULL_SIMP_TAC arith_ss []
+  ) >>
+
+  IMP_RES_TAC bir_exec_infinite_steps_fun_COUNT_PCs_LAST_STEP_thm >>
+  FULL_SIMP_TAC std_ss [] >>
+
+  PAT_X_ASSUM ``bir_state_COUNT_PC A B`` (K ALL_TAC) >>
+  PAT_X_ASSUM ``SUC A = B`` (fn thm => REWRITE_TAC [GSYM thm]) >>
+
+  Cases_on `n' = n''` >- (
+    FULL_SIMP_TAC arith_ss []
+  ) >>
+  `n' < n''` by (
+    FULL_SIMP_TAC arith_ss []
+  ) >>
+  FULL_SIMP_TAC std_ss [GSYM arithmeticTheory.LESS_EQ_IFF_LESS_SUC] >>
+  METIS_TAC [bir_exec_infinite_steps_fun_COUNT_PCs_GROWS_thm]
+);
+
+val bir_exec_step_state_PC_DIFF_IMP_Running_thm = store_thm(
+   "bir_exec_step_state_PC_DIFF_IMP_Running_thm", ``
+!bprog bs bs'.
+  (bir_exec_step_state bprog bs = bs') ==>
+  (bs.bst_pc <> bs'.bst_pc) ==>
+  (bs.bst_status = BST_Running /\ bs'.bst_status = BST_Running)
+``,
+  METIS_TAC [bir_exec_step_state_PC_DIFF_IMP_FINAL_Running_thm, bir_exec_step_state_FINAL_Running_IMP_INITIAL_Running_thm]
+);
+
+val bir_exec_infinite_steps_fun_NOT_terminated_thm = store_thm(
+   "bir_exec_infinite_steps_fun_NOT_terminated_thm", ``
+!bprog bs n L bs'.
+  (bir_exec_infinite_steps_fun bprog bs n = bs') ==>
+  (~(bir_state_is_terminated bs')) ==>
+  (!n'.
+    (n' < n) ==>
+    (~(bir_state_is_terminated (bir_exec_infinite_steps_fun bprog bs n'))))
+``,
+  Induct_on `n` >> (
+    FULL_SIMP_TAC std_ss [bir_exec_infinite_steps_fun_REWRS]
+  ) >>
+
+  FULL_SIMP_TAC std_ss [bir_state_is_terminated_def] >>
+  REPEAT STRIP_TAC >>
+
+  PAT_X_ASSUM ``!x.A`` (ASSUME_TAC o Q.SPECL [`bprog'`, `bir_exec_step_state bprog' bs`]) >>
+  REV_FULL_SIMP_TAC std_ss [] >>
+
+  Cases_on `n' = n` >- (
+    FULL_SIMP_TAC std_ss [bir_exec_infinite_steps_fun_COMM_thm] >>
+    METIS_TAC [bir_exec_step_state_FINAL_Running_IMP_INITIAL_Running_thm]
+  ) >>
+
+  `n' < n` by (
+    FULL_SIMP_TAC arith_ss []
+  ) >>
+
+  FULL_SIMP_TAC std_ss [bir_exec_infinite_steps_fun_COMM_thm] >>
+  METIS_TAC [bir_exec_step_state_FINAL_Running_IMP_INITIAL_Running_thm]
+);
+
+val bir_exec_infinite_steps_fun_LAST_PC_DIFF_IMP_Running_thm = store_thm(
+   "bir_exec_infinite_steps_fun_LAST_PC_DIFF_IMP_Running_thm", ``
+!bprog bs k bs'.
+  (bir_exec_infinite_steps_fun bprog bs (SUC k) = bs') ==>
+  ((bir_exec_infinite_steps_fun bprog bs k).bst_pc <> bs'.bst_pc) ==>
+  (bs.bst_status = BST_Running /\ bs'.bst_status = BST_Running)
+``,
+  FULL_SIMP_TAC std_ss [bir_exec_infinite_steps_fun_REWRS] >>
+  FULL_SIMP_TAC std_ss [bir_exec_infinite_steps_fun_COMM_thm] >>
+
+  REPEAT GEN_TAC >>
+  REPEAT DISCH_TAC >>
+  IMP_RES_TAC (SIMP_RULE std_ss [] bir_exec_step_state_PC_DIFF_IMP_Running_thm) >>
+  ASM_REWRITE_TAC [] >>
+
+  IMP_RES_TAC (SIMP_RULE std_ss [bir_state_is_terminated_def] bir_exec_infinite_steps_fun_NOT_terminated_thm) >>
+
+  Cases_on `k` >- (
+    FULL_SIMP_TAC std_ss [bir_exec_infinite_steps_fun_REWRS]
+  ) >>
+
+  PAT_X_ASSUM ``!x.A`` (ASSUME_TAC o Q.SPEC `0`) >>
+  FULL_SIMP_TAC arith_ss [bir_exec_infinite_steps_fun_REWRS]
+);
+
+val bir_exec_infinite_steps_fun_PC_DIFF_IMP_Running_thm = store_thm(
+   "bir_exec_infinite_steps_fun_PC_DIFF_IMP_Running_thm", ``
+!bprog bs n bs' L.
+  (bir_exec_infinite_steps_fun bprog bs n = bs') ==>
+  (n > 0) ==>
+  (!n'. n' < n ==> (bir_exec_infinite_steps_fun bprog bs n').bst_pc IN L) ==>
+  (bs'.bst_pc NOTIN L) ==>
+  (bs.bst_status = BST_Running /\ bs'.bst_status = BST_Running)
+``,
+  REPEAT GEN_TAC >>
+  REPEAT DISCH_TAC >>
+  Cases_on `n` >> (
+    FULL_SIMP_TAC arith_ss []
+  ) >>
+
+  `(bir_exec_infinite_steps_fun bprog' bs n').bst_pc <> bs'.bst_pc` by (
+    PAT_X_ASSUM ``!x.A`` (ASSUME_TAC o Q.SPEC `n'`) >>
+    FULL_SIMP_TAC arith_ss [] >>
+    REPEAT STRIP_TAC >>
+    FULL_SIMP_TAC (std_ss++pred_setSimps.PRED_SET_ss) [IN_APP]
+  ) >>
+  IMP_RES_TAC bir_exec_infinite_steps_fun_LAST_PC_DIFF_IMP_Running_thm >>
+  ASM_REWRITE_TAC []
+);
+
+val bir_exec_infinite_steps_fun_IMP_fun_COUNT_PCs_thm = store_thm(
+   "bir_exec_infinite_steps_fun_IMP_fun_COUNT_PCs_thm", ``
+!bprog bs n L bs'.
+  (bir_exec_infinite_steps_fun bprog bs n = bs') ==>
+  (n > 0) ==>
+  (bs'.bst_pc NOTIN L) ==>
+  (!n'.
+    (n' < n) ==>
+    ((bir_exec_infinite_steps_fun bprog bs n').bst_pc IN L)) ==>
+  (bir_exec_infinite_steps_fun_COUNT_PCs (F, {bs'.bst_pc}) bprog bs n = 1)
+``,
+  Cases_on `n` >- (
+    FULL_SIMP_TAC arith_ss []
+  ) >>
+  REPEAT STRIP_TAC >>
+  PAT_X_ASSUM ``SUC n' > 0`` (K ALL_TAC) >>
+  REPEAT (POP_ASSUM MP_TAC) >>
+  Q.ID_SPEC_TAC `bs'` >>
+  Q.ID_SPEC_TAC `L` >>
+  Q.ID_SPEC_TAC `n'` >>
+  Q.ID_SPEC_TAC `bs` >>
+
+  Induct_on `n'` >- (
+    REPEAT STRIP_TAC >>
+    FULL_SIMP_TAC std_ss [bir_exec_infinite_steps_fun_REWRS] >>
+
+    PAT_X_ASSUM ``!x.A`` (ASSUME_TAC o Q.SPEC `0`) >>
+    FULL_SIMP_TAC arith_ss [] >>
+    FULL_SIMP_TAC std_ss [bir_exec_infinite_steps_fun_REWRS] >>
+
+    `bs.bst_status = BST_Running /\
+     bs'.bst_status = BST_Running` by (
+      `bs.bst_pc <> bs'.bst_pc` by (
+        REPEAT STRIP_TAC >>
+        FULL_SIMP_TAC (std_ss++pred_setSimps.PRED_SET_ss) [IN_APP]
+      ) >>
+      IMP_RES_TAC bir_exec_step_state_PC_DIFF_IMP_Running_thm >>
+      ASM_SIMP_TAC std_ss []
+    ) >>
+
+    FULL_SIMP_TAC pure_ss [arithmeticTheory.ONE, bir_exec_infinite_steps_fun_COUNT_PCs_def] >>
+    FULL_SIMP_TAC (std_ss++holBACore_ss) [LET_DEF, bir_state_COUNT_PC_def] >>
+    FULL_SIMP_TAC std_ss [REWRITE_RULE [pred_setTheory.IN_APP] pred_setTheory.IN_SING]
+  ) >>
+
+  REPEAT STRIP_TAC >>
+  Q.ABBREV_TAC `k = SUC n'` >>
+
+  FULL_SIMP_TAC std_ss [bir_exec_infinite_steps_fun_REWRS] >>
+  FULL_SIMP_TAC pure_ss [bir_exec_infinite_steps_fun_COUNT_PCs_def] >>
+
+(*
+  FULL_SIMP_TAC pure_ss [bir_exec_infinite_steps_fun_COMM_thm] >>
+*)
+  Q.ABBREV_TAC `bs'' = bir_exec_step_state bprog' bs` >>
+  PAT_X_ASSUM ``!x y.A`` (ASSUME_TAC o Q.SPECL [`bs''`, `L`]) >>
+  REV_FULL_SIMP_TAC std_ss [] >>
+
+  `!n'. n' < k ==> (bir_exec_infinite_steps_fun bprog' bs'' n').bst_pc IN L` by (
+    REPEAT STRIP_TAC >>
+    PAT_X_ASSUM ``!x.A`` (ASSUME_TAC o Q.SPEC `SUC n''`) >>
+    REV_FULL_SIMP_TAC arith_ss [] >>
+    FULL_SIMP_TAC std_ss [bir_exec_infinite_steps_fun_REWRS] >>
+    METIS_TAC []
+  ) >>
+  FULL_SIMP_TAC std_ss [LET_DEF] >>
+
+  `bs''.bst_pc IN L` by (
+    Q.UNABBREV_TAC `k` >>
+    Q.UNABBREV_TAC `bs''` >>
+    REPEAT (PAT_X_ASSUM ``!x.A`` (ASSUME_TAC o Q.SPEC `1`)) >>
+    FULL_SIMP_TAC pure_ss [arithmeticTheory.ONE, bir_exec_infinite_steps_fun_REWRS, bir_exec_infinite_steps_fun_COMM_thm] >>
+    FULL_SIMP_TAC arith_ss []
+  ) >>
+
+  `bs''.bst_pc <> bs'.bst_pc` by (
+    REPEAT STRIP_TAC >>
+    FULL_SIMP_TAC (std_ss++pred_setSimps.PRED_SET_ss) [IN_APP]
+  ) >>
+
+  `k > 0` by (
+    Cases_on `k = 0` >- (
+      FULL_SIMP_TAC std_ss [bir_exec_infinite_steps_fun_REWRS] >>
+      REV_FULL_SIMP_TAC std_ss []
+    ) >>
+    FULL_SIMP_TAC arith_ss []
+  ) >>
+  IMP_RES_TAC bir_exec_infinite_steps_fun_PC_DIFF_IMP_Running_thm >>
+
+  FULL_SIMP_TAC pure_ss [arithmeticTheory.ONE, bir_exec_infinite_steps_fun_COUNT_PCs_def] >>
+  FULL_SIMP_TAC (std_ss++holBACore_ss) [LET_DEF, bir_state_COUNT_PC_def] >>
+  FULL_SIMP_TAC std_ss [REWRITE_RULE [pred_setTheory.IN_APP] pred_setTheory.IN_SING]
+);
+
+val bir_exec_infinite_steps_fun_IMP_COUNT_STEPS_thm = store_thm(
+   "bir_exec_infinite_steps_fun_IMP_COUNT_STEPS_thm", ``
+!bprog bs n L bs'.
+
+  (bir_exec_infinite_steps_fun bprog bs n = bs') ==>
+  (n > 0) ==>
+  (bs'.bst_pc NOTIN L) ==>
+  (!n'.
+    (n' < n) ==>
+    ((bir_exec_infinite_steps_fun bprog bs n').bst_pc IN L)) ==>
+
+(*
+(bs'.bst_pc.bpc_label IN ls) ==>
+(* TODO: need to add some more assumptions about ls in order to generalize this a bit *)
+*)
+
+  (bir_exec_infinite_steps_COUNT_STEPS (F, {bs'.bst_pc}) (SOME 1) bprog bs = SOME n)
+``,
+  REPEAT STRIP_TAC >>
+  IMP_RES_TAC bir_exec_infinite_steps_fun_IMP_fun_COUNT_PCs_thm >>
+
+  FULL_SIMP_TAC std_ss [bir_exec_infinite_steps_COUNT_STEPS_def] >>
+  REWRITE_TAC [whileTheory.OLEAST_EQ_SOME] >>
+  ASM_SIMP_TAC std_ss [] >>
+
+  IMP_RES_TAC bir_exec_infinite_steps_fun_PC_DIFF_IMP_Running_thm >>
+
+  REPEAT STRIP_TAC >- (
+    `~(bir_state_is_terminated bs')` by (
+      ASM_SIMP_TAC std_ss [bir_state_is_terminated_def]
+    ) >>
+    METIS_TAC [bir_exec_infinite_steps_fun_NOT_terminated_thm]
+  ) >>
+
+  `bir_state_COUNT_PC (F, {bs'.bst_pc}) (bir_exec_infinite_steps_fun bprog' bs n)` by (
+    FULL_SIMP_TAC (std_ss++holBACore_ss) [LET_DEF, bir_state_COUNT_PC_def, IN_SING, SING_applied]
+  ) >>
+
+  IMP_RES_TAC bir_exec_infinite_steps_fun_COUNT_PCs_LESS_STEPS_IMP_thm >>
+  FULL_SIMP_TAC arith_ss []
+);
+
+
+val bir_exec_infinite_steps_fun_IMP_exec_to_labels_thm = store_thm(
+   "bir_exec_infinite_steps_fun_IMP_exec_to_labels_thm", ``
+!bprog bs n L bs'.
+
+  (bir_exec_infinite_steps_fun bprog bs n = bs') ==>
+  (n > 0) ==>
+  (bs'.bst_pc NOTIN L) ==>
+  (!n'.
+    (n' < n) ==>
+    ((bir_exec_infinite_steps_fun bprog bs n').bst_pc IN L)) ==>
+
+  (bs'.bst_pc.bpc_index = 0) ==>
+
+  ?lo.
+  (bir_exec_to_labels {bs'.bst_pc.bpc_label} bprog bs = BER_Ended lo n 1 bs')
+``,
+  REWRITE_TAC
+    [bir_exec_to_labels_n_def, bir_exec_to_labels_def, bir_exec_steps_GEN_def] >>
+  REPEAT STRIP_TAC >>
+
+  `(\pc. pc.bpc_index = 0 /\ pc.bpc_label IN {bs'.bst_pc.bpc_label}) = {bs'.bst_pc}` by (
+    FULL_SIMP_TAC std_ss [EXTENSION, IN_SING, IN_APP] >>
+    REPEAT STRIP_TAC >>
+    EQ_TAC >> (
+      FULL_SIMP_TAC (std_ss++holBACore_ss) []
+    ) >>
+
+    Cases_on `x` >>
+    Cases_on `bs'.bst_pc` >>
+    FULL_SIMP_TAC (std_ss++holBACore_ss) []
+  ) >>
+  ASM_SIMP_TAC std_ss [] >>
+
+  IMP_RES_TAC bir_exec_infinite_steps_fun_IMP_COUNT_STEPS_thm >>
+  IMP_RES_TAC bir_exec_infinite_steps_fun_IMP_fun_COUNT_PCs_thm >>
+
+  FULL_SIMP_TAC (std_ss++holBACore_ss) [LET_DEF]
+);
+
+
+
+
+(*
+val bir_exec_to_labels_IMP_thm = store_thm(
+   "bir_exec_to_labels_IMP_thm", ``
+!L bprog bs lo n bs'.
+(bir_exec_to_labels L bprog bs = BER_Ended lo n 1 bs') ==>
+(!l. l IN L ==> IS_BL_Address l) ==>
+  ?n'.
+  (bir_exec_to_addr_label_n bprog bs n' = BER_Ended lo n n' bs')
+``,
+  REWRITE_TAC
+    [bir_exec_to_labels_n_def, bir_exec_to_labels_def, bir_exec_to_addr_label_n_def, bir_exec_steps_GEN_def] >>
+  REPEAT STRIP_TAC >>
+
+  FULL_SIMP_TAC std_ss [LET_DEF] >>
+  Cases_on `bir_exec_infinite_steps_COUNT_STEPS
+              (F,(\pc. pc.bpc_index = 0 /\ pc.bpc_label IN L)) (SOME 1) bprog'
+              bs` >> (
+    FULL_SIMP_TAC (std_ss++holBACore_ss) []
+  ) >>
+
+  cheat
+  (* TODO: this theorem might be not so useful because of the IS_BL_Address assumption *)
+);
+*)
+
+end;
+
+val bir_step_n_in_L_IMP_exec_infinite_steps_fun_thm0 = store_thm(
+   "bir_step_n_in_L_IMP_exec_infinite_steps_fun_thm0", ``
+!bprog bs n L bs'.
+  (step_n_in_L (\x. x.bst_pc) (bir_exec_step_state bprog) bs n L bs') ==>
+  (n > 0)
+``,
+  FULL_SIMP_TAC std_ss [step_n_in_L_def, step_n_in_L_relaxed_def]
+);
+
+val bir_step_n_in_L_IMP_exec_infinite_steps_fun_thm1 = store_thm(
+   "bir_step_n_in_L_IMP_exec_infinite_steps_fun_thm1", ``
+!bprog bs n L bs'.
+  (step_n_in_L (\x. x.bst_pc) (bir_exec_step_state bprog) bs n L bs') ==>
+  (bir_exec_infinite_steps_fun bprog bs n = bs')
+``,
+  FULL_SIMP_TAC std_ss [step_n_in_L_def, step_n_in_L_relaxed_def, bir_programTheory.bir_exec_infinite_steps_fun_def, step_n_def]
+);
+
+val bir_step_n_in_L_IMP_exec_infinite_steps_fun_thm2 = store_thm(
+   "bir_step_n_in_L_IMP_exec_infinite_steps_fun_thm2", ``
+!bprog bs n L bs'.
+  (step_n_in_L (\x. x.bst_pc) (bir_exec_step_state bprog) bs n L bs') ==>
+  (!n'.
+    (n' < n) ==>
+    ((bir_exec_infinite_steps_fun bprog bs n').bst_pc IN L))
+``,
+  FULL_SIMP_TAC std_ss [step_n_in_L_def, step_n_in_L_relaxed_def, bir_programTheory.bir_exec_infinite_steps_fun_def, step_n_def] >>
+
+  REPEAT STRIP_TAC >>
+  Cases_on `n' = 0` >- (
+    FULL_SIMP_TAC std_ss [arithmeticTheory.FUNPOW_0]
+  ) >>
+
+  `0 < n'` by (
+    FULL_SIMP_TAC arith_ss []
+  ) >>
+  METIS_TAC []
+);
+
+val bir_step_n_in_L_IMP_exec_to_labels_thm = store_thm(
+   "bir_step_n_in_L_IMP_exec_to_labels_thm", ``
+!bprog bs n L bs'.
+
+(step_n_in_L (\x. x.bst_pc) (bir_exec_step_state bprog) bs n L bs') ==>
+
+((bs'.bst_pc) NOTIN L) ==>
+(bs'.bst_pc.bpc_index = 0) ==>
+
+  ?lo.
+  (bir_exec_to_labels {bs'.bst_pc.bpc_label} bprog bs = BER_Ended lo n 1 bs')
+``,
+  REPEAT STRIP_TAC >>
+
+  IMP_RES_TAC bir_step_n_in_L_IMP_exec_infinite_steps_fun_thm0 >>
+  IMP_RES_TAC bir_step_n_in_L_IMP_exec_infinite_steps_fun_thm1 >>
+  IMP_RES_TAC bir_step_n_in_L_IMP_exec_infinite_steps_fun_thm2 >>
+
+  IMP_RES_TAC bir_exec_infinite_steps_fun_IMP_exec_to_labels_thm >>
+
+  METIS_TAC []
+);
+
+
+
+(*
+"bir_backlifterTheory.bir_exec_to_labels_TO_exec_to_addr_label_n"
+*)
+
+
+
+(*
+
+TODO: establish relational postcondition
+
+*)
+
+val abstract_jgmt_rel_def = Define `
+    abstract_jgmt_rel m (l:'a) (ls:'a->bool) pre post =
+  !ms .
+   ((m.pc ms) = l) ==> (pre ms) ==>
+   ?ms'. ((m.weak ms ls ms') /\
+    (post ms ms'))
+`;
+
+
+val bir_step_n_in_L_jgmt_TO_abstract_jgmt_rel_thm = prove (``
+!bprog l L ls pre post.
+(bir_step_n_in_L_jgmt
+  bprog
+  (bir_block_pc l)
+  L
+  pre
+  post) ==>
+
+(L INTER (IMAGE bir_block_pc ls) = EMPTY) ==>
+(!st st'. post st st' ==> st'.bst_pc IN (IMAGE bir_block_pc ls)) ==>
+
+(abstract_jgmt_rel
+  (bir_etl_wm bprog)
+  l
+  ls
+  pre
+  post)
+``,
+  cheat
+);
+
+
+val bir_abstract_jgmt_rel_thm = prove(``
+(abstract_jgmt_rel
+  (bir_etl_wm bprog)
+  (BL_Address (Imm32 2824w))
+  {BL_Address (Imm32 2886w)}
+  (\st.
+       st.bst_status = BST_Running /\
+       bir_envty_list_b birenvtyl st.bst_environ /\
+       bir_eval_exp
+         (BExp_BinExp BIExp_And
+            (BExp_BinExp BIExp_And
+               (BExp_BinPred BIExp_LessOrEqual (BExp_Const (Imm32 0xFFFFFFw))
+                  (BExp_Den (BVar "SP_process" (BType_Imm Bit32))))
+               (BExp_Aligned Bit32 2
+                  (BExp_Den (BVar "SP_process" (BType_Imm Bit32)))))
+            (BExp_BinPred BIExp_LessOrEqual
+               (BExp_Den (BVar "countw" (BType_Imm Bit64)))
+               (BExp_Const (Imm64 0xFFFFFFFFFFFFFF00w)))) st.bst_environ =
+       SOME bir_val_true)
+  (\st st'.
+         ?v1 v2.
+           bir_env_lookup "countw" st.bst_environ =
+           SOME (BVal_Imm (Imm64 v1)) /\
+           bir_env_lookup "countw" st'.bst_environ =
+           SOME (BVal_Imm (Imm64 v2)) /\
+           v1 <+ v2 /\
+           v1 + 44w <=+ v2 /\
+           v2 <=+ v1 + 47w))
+``,
+  cheat
+);
+
+(*
+
+TODO: transfer of relational postcondition to machine model
+
+*)
+
+
+(*
+TODO: go to didrik style m0_mod weak transition relation
+*)
+
+val m_weak_trs_def = Define `
+    m_weak_trs pcf stepf ms ls ms' = 
+        ?n.
+          ((n > 0) /\
+           (FUNPOW_OPT stepf n ms = SOME ms') /\
+           ((pcf ms') IN ls)
+          ) /\
+          !n'.
+            (((n' < n) /\ (n' > 0)) ==>
+            ?ms''.
+              (FUNPOW_OPT stepf n' ms = SOME ms'') /\
+              ((pcf ms'') NOTIN ls)
+            )`;
+val m_weak_model_def = Define `
+    m_weak_model pcf bmr  = <|
+    trs  := bmr.bmr_step_fun;
+    weak := m_weak_trs pcf bmr.bmr_step_fun;
+    pc   := pcf
+  |>`;
+val m0_mod_weak_trs_def = Define `
+    m0_mod_weak_trs = m_weak_trs (\x. x.base.REG RName_PC) (m0_mod_bmr (T,T)).bmr_step_fun
+`;
+val m0_mod_weak_model_def = Define `
+    m0_mod_weak_model = m_weak_model (\x. x.base.REG RName_PC) (m0_mod_bmr (T,T))
+`;
+
+val m_triple_rel_def = Define `
+    m_triple_rel wm bmr mms l ls pre post =
+    abstract_jgmt_rel wm l ls
+      (\ms. (bmr.bmr_extra ms)  /\
+            (EVERY (bmr_ms_mem_contains bmr ms) mms) /\
+            (pre ms))         
+      (\ms ms'. (bmr.bmr_extra ms')  /\
+            (EVERY (bmr_ms_mem_contains bmr ms') mms) /\
+            (post ms ms'))
+`;
+val m0_mod_triple_rel_def = Define `
+    m0_mod_triple_rel = m_triple m0_mod_weak_model (m0_mod_bmr (T,T))
+`;
 
 (* TODO: translate to pure Cortex-M0 property *)
+(* =================================================================================== *)
 (*
 bir_backlifterTheory.bir_post_bir_to_arm8_def
 lift_contract_thm
@@ -499,6 +1561,7 @@ get_arm8_contract_sing
 
 examples/tutorial/7-composition/tutorial_backliftingScript.sml
 *)
+(* =================================================================================== *)
 
 (* TODO: stolen and adjusted/generalized from "bir_backlifterTheory.bir_is_lifted_prog_MULTI_STEP_EXEC_compute" *)
 (* =================================================================================== *)
@@ -541,42 +1604,61 @@ val bir_is_lifted_prog_MULTI_STEP_EXEC_compute_32_8_thm =
 
 
 (*
+
+TODO: this is probably in precondition lifting
+"bir_backlifterTheory.exist_bir_of_arm8_thm"
+bir_backlifterTheory.bir_pre_arm8_to_bir_def
+bir_backlifterTheory.bir_post_bir_to_arm8_def
+((
 !ms.
 ?bs.
-  bmr_rel (r) bs ms
-arm8_bmr
-m0_mod_bmr
+  (bir_envty_list_b birenvtyl st.bst_environ) /\
+  bmr_rel (m0_mod_bmr (T,T)) bs ms
+))
+bir_lifting_machinesTheory.m0_mod_bmr_def
 
 
 
+((
+``
 !bprog bs n L bs'.
 (step_n_in_L (\x. x.bst_pc) (bir_exec_step_state bprog) bs n L bs') ==>
   ?n' lo.
   (bir_exec_to_addr_label_n bprog bs n' = BER_Ended lo n n' bs')
+``
+))
+*)
 
 
 
 
-!bprog bs n L bs'.
-(step_n_in_L (\x. x.bst_pc) (bir_exec_step_state bprog) bs n L bs') ==>
-((bs'.bst_pc) NOTIN L) ==>
-(bs'.bst_pc.bpc_index = 0) ==>
-  ?lo.
-  (bir_exec_to_labels {bs'.bst_pc.bpc_label} bprog bs = BER_Ended lo n 1 bs')
+val lift_contract_thm = store_thm(
+   "lift_contract_thm", ``
+!mla.
+  bir_is_lifted_prog (m0_mod_bmr (T,T)) mu mms p ==>
+  (MEM (BL_Address mla) (bir_labels_of_program bprog)) ==>
+
+  (abstract_jgmt_rel
+    (bir_etl_wm bprog)
+    (BL_Address (Imm32 l))
+    (IMAGE (\x. (BL_Address (Imm32 x))) ls)
+    (bpre)
+    (bpost)) ==>
+
+  (abstract_jgmt_rel
+    m0_mod_weak_model
+    l
+    ls
+    (m0_mod_pre)
+    (m0_mod_post))
+``,
+  cheat
+);
 
 
+(*
 
-(bir_exec_to_labels L bprog bs = BER_Ended lo n n' bs') ==>
-  ?n''.
-  (bir_exec_to_addr_label_n bprog bs n' = BER_Ended lo n n'' bs')
-
-
-
-TODO: go to didrik style m0_mod weak transition relation
-
-TODO: transfer to relational postcondition
-
-TODO: transfer to m0 model (unmodified)
+TODO: transfer to (unmodified) m0 model
 
 *)
 
